update

theory/JITPer_aux.thy
@@ -244,15 +244,15 @@ definition per_jit_load_reg64 :: "bpf_ireg \<Rightarrow> bpf_ireg \<Rightarrow> 
 "per_jit_load_reg64 dst src chk off = (
   let l_bin = 
     x64_encode (Pmovl_ri R11 (scast off))@x64_encode (Paddq_rr R11 (bpf_to_x64_reg src))@
-    x64_encode (Pmov_mr (Addrmode (Some R11) None 0) (bpf_to_x64_reg dst) chk) in
+    x64_encode (Pmov_rm (bpf_to_x64_reg dst) (Addrmode (Some R11) None 0) chk) in
     Some (3, 0, l_bin)
 )"
 
 definition per_jit_store_reg64 :: "bpf_ireg \<Rightarrow> bpf_ireg \<Rightarrow> memory_chunk \<Rightarrow> off_ty \<Rightarrow> (nat \<times> u64 \<times> x64_bin) option" where
 "per_jit_store_reg64 dst src chk off = (
   let l_bin = 
-    x64_encode (Pmovq_ri R11 (scast off))@x64_encode (Paddq_rr R11 (bpf_to_x64_reg dst))@
-    x64_encode (Pmovq_rr R10 (bpf_to_x64_reg src))@x64_encode (Pmov_rm R10 (Addrmode (Some R11) None 0) chk) in
+    x64_encode (Pmovl_ri R11 (scast off))@x64_encode (Paddq_rr R11 (bpf_to_x64_reg dst))@
+    x64_encode (Pmovq_rr R10 (bpf_to_x64_reg src))@x64_encode (Pmov_mr (Addrmode (Some R11) None 0) R10 chk) in
     Some (4, 0, l_bin)
 )"
 
