theory/x64Semantics.thy
@@ -149,7 +149,7 @@ definition exec_instr :: "instruction \<Rightarrow> nat \<Rightarrow> nat \<Righ
   Pcmpq_rr rd r1 \<Rightarrow> Next (pc+sz)(compare_longs (rs (IR r1)) (rs (IR rd)) rs) m ss |
   Pmovq_ri rd n  \<Rightarrow> Next (pc + sz) (rs#(IR rd) <- n) m ss |
   Pmovl_ri rd n   \<Rightarrow> Next (pc + sz) (rs#(IR rd) <- (scast n)) m ss|    \<comment> \<open> load imm32 to reg \<close>
-  Pmov_mr  a r1 c \<Rightarrow> exec_load pc sz c m ss a rs (IR r1) |                    
+  Pmov_mr  a r1 c \<Rightarrow> exec_store pc sz c m ss a rs (IR r1) |                    
   Pxchgq_rr rd r1 \<Rightarrow> let tmp = rs (IR rd) in
                      let rs1 = (rs#(IR rd)<- (rs (IR r1))) in
                        Next (pc + sz) (rs1#(IR r1)<- tmp) m ss |
@@ -157,7 +157,7 @@ definition exec_instr :: "instruction \<Rightarrow> nat \<Rightarrow> nat \<Righ
   Pshrq_r   rd    \<Rightarrow> Next (pc + sz) (rs#(IR rd) <- ((rs (IR rd))>> (unat (and ( (ucast (rs(IR RCX)))::u32) (63::u32))))) m ss |
   Psarq_r   rd    \<Rightarrow> Next (pc + sz) (rs#(IR rd) <- (ucast (arsh64 ((scast (rs (IR rd)))::i64) (unat (and ( (ucast (rs(IR RCX)))::u32) (63::u32)))))) m ss |
 \<comment> \<open>TODO  Psarq_r   rd    \<Rightarrow> Next (pc + sz) (rs#(IR rd) <- (ucast (((scast (rs (IR rd)))::i64) >> (unat (and ( (ucast (rs(IR RCX)))::u32) (63::u32)))))) m ss | \<close>
-  Pmov_rm  rd a c \<Rightarrow> exec_store pc sz c m ss a rs (IR rd) |            \<comment> \<open> store reg to mem \<close>
+  Pmov_rm  rd a c \<Rightarrow> exec_load pc sz c m ss a rs (IR rd) |            
   Pcall_i   n   \<Rightarrow> exec_call pc sz M64 m ss rs n
 )"
 (*Ptestq_rr r1 r2 \<Rightarrow> Next (pc+sz) (compare_longs (and (rs (IR r1)) (rs (IR r2))) 0 rs) m ss*)
